Lynx.lean
@@ -1,4 +1,6 @@
-import Lynx.Term
-import Lynx.Modules.Erlang
-import Lynx.Modules.Maps
-import Lynx.Tactic
+module
+
+public import Lynx.Term
+public import Lynx.Modules.Erlang
+public import Lynx.Modules.Maps
+public import Lynx.Tactic
