Lynx/Modules/Erlang.lean
@@ -1,3 +1,5 @@
-import Lynx.Modules.Erlang.Fun
-import Lynx.Modules.Erlang.Guards
-import Lynx.Modules.Erlang.Process
+module
+
+public import Lynx.Modules.Erlang.Fun
+public import Lynx.Modules.Erlang.Guards
+public import Lynx.Modules.Erlang.Process
